# Answers for Exam-2




#### **Find the zeroes of the quadratic polynomial $x^2+ 7x + 10$, and verify the relationship between the zeroes and the coefficients.**

Steps to solve:
**1. Use the quadratic formula:**
$$x = \frac{-b \pm \sqrt{b^2 - 4ac}}{2a}$$
where a, b, and c are the coefficients of the quadratic equation. In this case, a = 1, b = 7, and c = 10. Substituting these values into the formula, we get:
$$x = \frac{-7 \pm \sqrt{7^2 - 4 \cdot 1 \cdot 10}}{2 \cdot 1}$$
$$x = \frac{-7 \pm \sqrt{9}}{2}$$

**2. Simplify:**
$$x = \frac{-7 \pm 3}{2}$$

**3. Separate the equations and solve:**
$$x = -2$$
$$x = -5$$

**Answer:**
The zeroes of the quadratic polynomial $x^2+7x+10$ are **x = -2** and **x = -5**.

**Verification of the relationship between the zeroes and the coefficients:**
According to Vieta's formulas, the sum of the zeroes of a quadratic equation is equal to the negative of the coefficient b divided by a, and the product of the zeroes is equal to c divided by a. In this case, we can verify that:

* Sum of zeroes: (-2) + (-5) = -7 = -b/a
* Product of zeroes: (-2) * (-5) = 10 = c/a

Therefore, the relationship between the zeroes and the coefficients is verified.

#### **Find the roots of the quadratic equation $3x^2 - 2 \sqrt{6}x+ 2 = 0$**

      
  1. **Identify the coefficients:**
     - $a = 3$
     - $b = -2\sqrt{6}$
     - $c = 2$
  
  2. **Apply the quadratic formula:**
     $$x = \dfrac{-b \pm \sqrt{b^2 - 4ac}}{2a}$$
  
  3. **Substitute the coefficients:**
     $$x = \dfrac{+2\sqrt{6} \pm \sqrt{(-2\sqrt{6})^2 - 4 \cdot 3 \cdot 2}}{2 \cdot 3}$$
  
  4. **Simplify the expression under the radical:**
     $$x = \dfrac{2\sqrt{6} \pm \sqrt{24 - 24}}{6}$$
     $$x = \dfrac{2\sqrt{6} \pm \sqrt{0}}{6}$$
  
  5. **Reduce the expression:**
     $$x = \dfrac{2\sqrt{6}}{6}$$
  
  6. **Simplify the fraction:**
     $$x = \dfrac{\sqrt{6}}{3}$$
  
  **Therefore, the quadratic equation $3x^2 - 2 \sqrt{6}x+ 2 = 0$ has a single root, which is $x = \dfrac{\sqrt{6}}{3}$.**


